code/ecdsap256/Hacl.P256.fsti
@@ -20,6 +20,152 @@ open Hacl.Impl.P256.Compression
 open Spec.P256.MontgomeryMultiplication
 
 
+val toFormPoint: i: lbuffer uint8 (size 64) -> result: point -> Stack unit 
+  (requires fun h -> live h i /\ live h result /\ disjoint i result)
+  (ensures fun h0 _ h1 -> modifies (loc result) h0 h1 /\ (
+    let pointScalarXSeq = nat_from_bytes_be (as_seq h0 (gsub i (size 0) (size 32))) in 
+    let pointScalarYSeq = nat_from_bytes_be (as_seq h0 (gsub i (size 32) (size 32))) in 
+    let x, y, z = point_prime_to_coordinates (as_seq h1 result) in 
+    let pointJacX, pointJacY, pointJacZ = toJacobianCoordinates (pointScalarXSeq, pointScalarYSeq) in 
+    x == pointScalarXSeq /\ y == pointScalarYSeq /\ z == 1 /\
+    x == pointJacX /\ y == pointJacY /\ z == pointJacZ))
+
+
+val fromFormPoint: i: point -> o: lbuffer uint8 (size 64) -> Stack unit
+  (requires fun h -> live h i /\ live h o /\ disjoint i o /\
+    as_nat h (gsub i (size 0) (size 4)) < prime256 /\
+    as_nat h (gsub i (size 4) (size 4)) < prime256 )
+  (ensures fun h0 _ h1 -> modifies (loc i |+| loc o) h0 h1 /\ (
+    let xCoordinate = gsub i (size 0) (size 4) in 
+    let yCoordinate = gsub i (size 4) (size 4) in 
+
+    let scalarX = gsub o (size 0) (size 32) in 
+    let scalarY = gsub o (size 32) (size 32) in 
+
+    as_seq h1 scalarX == nat_to_bytes_be 32 (as_nat h0 xCoordinate) /\
+    as_seq h1 scalarY == nat_to_bytes_be 32 (as_nat h0 yCoordinate)))
+
+
+val secretToPublic:
+    result:lbuffer uint8 (size 64)
+  -> scalar:lbuffer uint8 (size 32)
+  -> Stack bool
+  (requires fun h ->
+    live h result /\ live h scalar /\ 
+    disjoint result scalar)
+  (ensures fun h0 r h1 ->
+    let pointX, pointY, flag = ecp256_dh_i (as_seq h0 scalar) in
+    modifies (loc result) h0 h1 /\
+    r == flag /\
+    as_seq h1 (gsub result (size 0) (size 32)) == pointX /\
+    as_seq h1 (gsub result (size 32) (size 32)) == pointY)
+
+
+
+val secretToPublicRaw:
+    result:lbuffer uint8 (size 64)
+  -> scalar:lbuffer uint8 (size 32)
+  -> Stack unit
+  (requires fun h ->
+    live h result /\ live h scalar /\ 
+    disjoint result scalar)
+  (ensures fun h0 r h1 ->
+    modifies (loc result) h0 h1 /\ (
+    let (xN, yN, zN) = secret_to_public (as_seq h0 scalar)  in 
+
+    let scalarX = gsub result (size 0) (size 32) in 
+    let scalarY = gsub result (size 32) (size 32) in 
+
+    as_seq h1 scalarX == nat_to_bytes_be 32 xN /\
+    as_seq h1 scalarY == nat_to_bytes_be 32 yN))
+
+
+
+val scalarMult:
+    result:lbuffer uint8 (size 64)
+  -> pubKey:lbuffer uint8 (size 64)
+  -> scalar:lbuffer uint8 (size 32)
+  -> Stack bool
+    (requires fun h ->
+      live h result /\ live h pubKey /\ live h scalar /\
+      disjoint result pubKey /\ disjoint result scalar)
+    (ensures fun h0 r h1 ->
+      let pubKeyX = gsub pubKey (size 0) (size 32) in
+      let pubKeyY = gsub pubKey (size 32) (size 32) in
+      let pointX, pointY, flag =
+        ecp256_dh_r (as_seq h0 pubKeyX) (as_seq h0 pubKeyY) (as_seq h0 scalar) in
+      r == flag /\
+      modifies (loc result) h0 h1 /\
+      as_seq h1 (gsub result (size 0) (size 32)) == pointX /\
+      as_seq h1 (gsub result (size 32) (size 32)) == pointY)
+
+
+val scalarMultRaw:
+    result:lbuffer uint8 (size 64)
+  -> pubKey:lbuffer uint8 (size 64)
+  -> scalar:lbuffer uint8 (size 32)
+  -> Stack unit
+    (requires fun h ->
+      live h result /\ live h pubKey /\ live h scalar /\
+      disjoint result pubKey /\ disjoint result scalar /\ (
+      let x, y = gsub pubKey (size 0) (size 32), gsub pubKey (size 32) (size 32) in 
+      nat_from_bytes_be (as_seq h x) < prime256 /\
+      nat_from_bytes_be (as_seq h y) < prime256))
+    (ensures fun h0 _ h1 -> modifies (loc result |+| loc pubKey) h0 h1 /\ (
+      let pointScalarXSeq = nat_from_bytes_be (as_seq h0 (gsub pubKey (size 0) (size 32))) in 
+      let pointScalarYSeq = nat_from_bytes_be (as_seq h0 (gsub pubKey (size 32) (size 32))) in  
+      let pointJacX, pointJacY, pointJacZ = toJacobianCoordinates (pointScalarXSeq, pointScalarYSeq) in 
+      let (xN, yN, zN) = scalar_multiplication (as_seq h0 scalar) (pointJacX, pointJacY, pointJacZ ) in 
+      let scalarX = gsub result (size 0) (size 32) in 
+      let scalarY = gsub result (size 32) (size 32) in 
+  
+      as_seq h1 scalarX == nat_to_bytes_be 32 xN /\
+      as_seq h1 scalarY == nat_to_bytes_be 32 yN
+    )
+  )
+
+
+val ecdsa_verification_point_operations: result: lbuffer uint8 (size 32) -> publicKey: lbuffer uint8 (size 64) -> 
+  u1: lbuffer uint8 (size 32) -> u2: lbuffer uint8 (size 32) ->
+  Stack bool 
+  (requires fun h -> live h result /\ live h publicKey /\ live h u1 /\ live h u2 /\
+    LowStar.Monotonic.Buffer.all_disjoint [loc result; loc publicKey; loc u1; loc u2] /\ (
+    let publicKeyX = nat_from_bytes_be (as_seq h (gsub publicKey (size 0) (size 32))) in
+    let publicKeyY = nat_from_bytes_be (as_seq h (gsub publicKey (size 32) (size 32))) in 
+    publicKeyX < prime256 /\ publicKeyY < prime256 ))
+  (ensures fun h0 r h1 -> modifies (loc result) h0 h1 /\ (
+    let pointScalarXSeq = nat_from_bytes_be (as_seq h0 (gsub publicKey (size 0) (size 32))) in 
+    let pointScalarYSeq = nat_from_bytes_be (as_seq h0 (gsub publicKey (size 32) (size 32))) in 
+    let pubJac = toJacobianCoordinates (pointScalarXSeq, pointScalarYSeq) in 
+    let pointAtInfinity = (0, 0, 0) in
+    let u1D, _ = montgomery_ladder_spec (as_seq h0 u1) (pointAtInfinity, basePoint) in
+    let u2D, _ = montgomery_ladder_spec (as_seq h0 u2) (pointAtInfinity, pubJac) in
+    let sumD = if  _norm u1D =  _norm u2D then  _point_double u1D else  _point_add u1D u2D in 
+    let pointNorm = _norm sumD in
+    let (xResult, yResult, zResult) = pointNorm in
+    r == not (Spec.P256.isPointAtInfinity pointNorm) /\
+    as_seq h1 result == nat_to_bytes_be 32  (xResult % prime_p256_order)))
+
+
+
+
+
+
+
+
+
+
+
+
+
+
+
+
+
+
+
+
+
 [@ (Comment " Input: result buffer: uint8[64], \n m buffer: uint8 [mLen], \n priv(ate)Key: uint8[32], \n k (nonce): uint32[32]. 
   \n Output: bool, where True stands for the correct signature generation. False value means that an error has occurred. 
   \n The private key and the nonce are expected to be more than 0 and less than the curve order.")]
